将两个有序链表合并为一个新的有序链表并返回。新链表是通过拼接给定的两个链表的所有节点组成的。 

示例：

输入：

```
1->2->4, 1->3->4
```

输出：

```
1->1->2->3->4->4
```



#### python解法1	

```python
class Solution(object):
	    def mergeTwoLists(self, l1, l2):
	        """
	        :type l1: ListNode
	        :type l2: ListNode
	        :rtype: ListNode
	        """
	        curr=dummy=ListNode(0)
	        while l1 and l2:
	            if l1.val<l2.val:
	                curr.next=l1
	                l1=l1.next
	            else:
	                curr.next=l2
	                l2=l2.next
	            curr=curr.next
	        curr.next=l1 or l2
	        return dummy.next
```

#### python解法2	

```python
class Solution(object):
    def mergeTwoLists(self, l1, l2):
        """
        :type l1: ListNode
        :type l2: ListNode
        :rtype: ListNode
        """
        curr=ListNode(-1)
        head=curr
        while l2 != None:
            while l1!= None and l1.val<l2.val:
                head.next=l1
                l1=l1.next
                head=head.next
            head.next=l2
            head=head.next
            l2=l2.next
        head.next = l1 if l1 != None else l2
        return curr.next
```

#### java解法1

```java
class Solution {
    public ListNode mergeTwoLists(ListNode l1, ListNode l2) {
        ListNode curr=new ListNode(0);
        ListNode head=curr;
        while (l1!=null && l2!=null){
            if(l1.val<l2.val){
                curr.next=l1;
                l1=l1.next;
            }else {
                curr.next=l2;
                l2=l2.next;
            }
            curr=curr.next;
        } 
        curr.next = l1!=null ? l1 : l2;
        return head.next;
        }
}
```

